* coq/junk/CatSemEx/falg_initial_iso.v:

coq/junk/CatSemEx/falg.v
@@ -9,19 +9,19 @@ Section FAlgebra.
 Variable C:Cat.
 Variable F:Functor C C.
 
-Record F_Algebra :=
-{ F_Algebra_obj :> C
-; F_Algebra_alg :> F F_Algebra_obj ---> F_Algebra_obj
+Record FAlg :=
+{ FAlg_obj :> C
+; FAlg_alpha : F FAlg_obj ---> FAlg_obj
 }.
 
-Record F_Algebra_mor (FA FB:F_Algebra) :=
-  { F_Algebra_mor_mor :> FA ---> FB
-  ; F_Algebra_mor_prop : comp (Cat_struct:=C)  FA (F_Algebra_mor_mor) == #F F_Algebra_mor_mor ;; FB}.
+Record FAlg_map (FA FB:FAlg) :=
+  { FAlg_map_mor :> FA ---> FB
+  ; FAlg_map_prop : FAlg_alpha FA ;; FAlg_map_mor == #F FAlg_map_mor ;; FAlg_alpha FB}.
 
-Infix "--->_F" := F_Algebra_mor (at level 60, right associativity).
+Infix "--->_F" := FAlg_map (at level 60, right associativity).
 
-Program Instance F_Algebra_mor_oid (FA FB:F_Algebra) : Setoid (FA --->_F FB) :=
-  { equiv f g := (F_Algebra_mor_mor f) == g }.
+Program Instance F_Algebra_mor_oid (FA FB:FAlg) : Setoid (FA --->_F FB) :=
+  { equiv f g := FAlg_map_mor f == g }.
 Next Obligation.
 intros a b.
 split.
@@ -32,24 +32,23 @@ split.
   intros f g h H0 H1; etransitivity; eauto.
 Qed.
 
-Definition F_Algebra_mor_id (A:F_Algebra) : A --->_F A.
-split with (id (F_Algebra_obj A)).
+Definition F_Algebra_mor_id (A:FAlg) : A --->_F A.
+exists (id (FAlg_obj A)).
 cat.
 Defined.
 
-Definition F_Algebra_mor_comp (a b c:F_Algebra) (f: a --->_F b) (g: b --->_F c) : a --->_F c.
-split with (F_Algebra_mor_mor f ;; g).
-pose (H:=comp_oid (Cat_struct:=C)).
+Definition F_Algebra_mor_comp (a b c:FAlg) (f: a --->_F b) (g: b --->_F c) : a --->_F c.
+exists (FAlg_map_mor f ;; g).
 rewrite <- assoc.
-rewrite (F_Algebra_mor_prop f).
+rewrite (FAlg_map_prop f).
 rewrite assoc.
 rewrite (preserve_comp (Functor_struct:=F)).
-rewrite (F_Algebra_mor_prop g).
+rewrite (FAlg_map_prop g).
 rewrite assoc.
 reflexivity.
 Defined.
 
-Program Instance F_Algebra_Cat_struct : Cat_struct F_Algebra_mor :=
+Program Instance F_Algebra_Cat_struct : Cat_struct FAlg_map :=
 { mor_oid := F_Algebra_mor_oid 
 ; id := F_Algebra_mor_id
 ; comp := F_Algebra_mor_comp }.
@@ -57,8 +56,7 @@ Solve Obligations using cat.
 Next Obligation.
 intros a b c f g H0 h i H1.
 simpl in *.
-rewrite H0; rewrite H1.
-reflexivity.
+apply comp_oid; assumption.
 Qed.
 Next Obligation.
 intros a b c d f g h.
